steel/Learn.Steel.ListP.Impl.fst
@@ -1,0 +1,195 @@
+module Learn.Steel.ListP.Impl
+
+module L   = FStar.List.Pure
+module G   = FStar.Ghost
+module US  = Learn.Steel.Util
+module U32 = FStar.UInt32
+module Loops = Steel.Loops (* Not yet extracted by krml ? *)
+
+open Steel.Effect
+open Steel.Effect.Atomic
+open Steel.FractionalPermission
+open Steel.Reference
+
+open Learn.Steel.ListP.Param
+open Learn.Steel.ListP.Data
+open Learn.Steel.ListP.Derived
+
+#set-options "--fuel 3 --ifuel 1"
+
+(* [length] *)
+
+let length_ty (p : list_param) : Type = (r : ref p.r) ->
+  Steel  U32.t
+        (mlistN p r) (fun _ -> mlistN p r)
+        (requires fun h0        -> L.length (sel_listN p r h0) <= FStar.UInt.max_int U32.n)
+        (ensures  fun h0 len h1 -> frame_equalities (mlistN p r) h0 h1 /\
+                                U32.v len = L.length (sel_listN p r h0))
+
+inline_for_extraction noextract
+let length_body (p : list_param) ($rec_f : length_ty p) : length_ty p
+  = fun r ->
+    let b = listN_is_nil p r in
+    if b
+    then return 0ul
+    else begin
+      let r'   = listN_next p r in
+      let len' = rec_f r'       in
+      (**) intro_mlistN_cons p r r';
+      return U32.(len' +^ 1ul)
+    end
+
+(* [reverse] *)
+
+unfold let reverse_inv_vp1 (p : list_param) (rs : ref p.r & ref p.r) : vprop =
+  mlistN p rs._1 `star` mlistN p rs._2
+
+let reverse_inv_ref (p : list_param) (trg : list (cell_t p)) (b : G.erased bool)
+  (s : (rs : (ref p.r & ref p.r) & (mlistN_sel_t p rs._1 & mlistN_sel_t p rs._2)))
+  : prop =
+  trg == L.rev_acc s._2._1 s._2._2 /\ is_null s._1._1 = not (G.reveal b)
+
+let reverse_inv (p : list_param) (trg : list (cell_t p)) (it_f it_r : ref (ref p.r))
+                (b : G.erased bool) : vprop =
+  vrefine ((vptr it_f `star` vptr it_r) `vdep` reverse_inv_vp1 p)
+          (reverse_inv_ref p trg b)
+
+let reverse_inv_def (p : list_param) (trg : list (cell_t p)) (it_f it_r : ref (ref p.r)) (b : G.erased bool)
+  : squash (reverse_inv p trg it_f it_r b ==
+            vrefine ((vptr it_f `star` vptr it_r) `vdep` reverse_inv_vp1 p) (reverse_inv_ref p trg b))
+  = ()
+
+let intro_reverse_inv #opened (p : list_param) trg it_f it_r (b : G.erased bool) (r_f r_r : ref p.r)
+  : SteelGhost unit opened
+              (vptr it_f `star` vptr it_r `star` mlistN p r_f `star` mlistN p r_r)
+              (fun () -> reverse_inv p trg it_f it_r b)
+              (requires fun h -> sel it_f h == r_f /\ sel it_r h == r_r /\
+                              trg == L.rev_acc (sel_listN p r_f h) (sel_listN p r_r h) /\
+                              is_null r_f = not (G.reveal b))
+              (ensures fun _ _ _ -> True)
+  =
+    intro_vdep (vptr it_f `star` vptr it_r)
+               (mlistN p r_f `star` mlistN p r_r)
+               (reverse_inv_vp1 p);
+    intro_vrefine ((vptr it_f `star` vptr it_r) `vdep` reverse_inv_vp1 p)
+                  (reverse_inv_ref p trg b)
+
+let elim_reverse_inv #opened (p : list_param) (trg : list (cell_t p)) (it_f it_r : ref (ref p.r))
+                             (b : G.erased bool)
+  : SteelGhost (G.erased (ref p.r & ref p.r)) opened
+               (reverse_inv p trg it_f it_r b)
+               (fun rs -> vptr it_f `star` vptr it_r `star` reverse_inv_vp1 p rs)
+               (requires fun _ -> True)
+               (ensures fun _ rs h ->
+                 sel it_f h == (G.reveal rs)._1 /\
+                 sel it_r h == (G.reveal rs)._2 /\
+                (let ls = h (reverse_inv_vp1 p rs) in
+                 trg == L.rev_acc ls._1 ls._2) /\
+                 is_null (G.reveal rs)._1 = not (G.reveal b))
+  = 
+    elim_vrefine ((vptr it_f `star` vptr it_r) `vdep` reverse_inv_vp1 p)
+                 (reverse_inv_ref p trg b);
+    elim_vdep (vptr it_f `star` vptr it_r) (reverse_inv_vp1 p)
+
+let elim_reverse_inv_vp1 #opened (p : list_param) (rs : ref p.r & ref p.r) (r_f r_r : ref p.r)
+  : SteelGhost unit opened
+               (reverse_inv_vp1 p rs) (fun () -> mlistN p r_f `star` mlistN p r_r)
+               (requires fun _ -> rs == (r_f, r_r))
+               (ensures fun h0 () h1 -> rs == (r_f, r_r) /\
+                                     h0 (reverse_inv_vp1 p rs) == (sel_listN p r_f h1, sel_listN p r_r h1))
+  =
+    change_equal_slprop (reverse_inv_vp1 p rs) (reverse_inv_vp1 p rs); (*TODO: why is it necessary?*)
+    change_equal_slprop (reverse_inv_vp1 p rs)
+                        (mlistN p r_f `star` mlistN p r_r)
+
+inline_for_extraction noextract
+let reverse_loop_cond (p : list_param) (trg : G.erased (list (cell_t p))) it_f it_r ()
+  : SteelT bool (h_exists (reverse_inv p trg it_f it_r)) (fun b -> reverse_inv p trg it_f it_r b)
+  =
+    (**) let gb' : G.erased (G.erased bool) = witness_exists () in
+    (**) let gb  : G.erased bool = G.reveal gb' in
+    (**) change_equal_slprop (reverse_inv p trg it_f it_r (G.reveal gb'))
+    (**)                     (reverse_inv p trg it_f it_r gb);
+    (**) let rs   = elim_reverse_inv p trg it_f it_r gb in
+    (**) let gr_f = G.hide (G.reveal rs)._1 in
+    (**) let gr_r = G.hide (G.reveal rs)._2 in
+    let r_f = read it_f in
+    (**) elim_reverse_inv_vp1 p rs r_f gr_r;
+    (**) intro_reverse_inv p trg it_f it_r (not (is_null r_f)) r_f gr_r;
+    return (not (is_null r_f))
+
+inline_for_extraction noextract
+let reverse_loop_body (p : list_param) (trg : G.erased (list (cell_t p))) (it_f it_r : ref (ref p.r)) ()
+  : SteelT unit (reverse_inv p trg it_f it_r true)
+                (fun () -> h_exists (reverse_inv p trg it_f it_r))
+  =
+    (**) let rs = elim_reverse_inv p trg it_f it_r true in
+    let r_f = read it_f in
+    let r_r = read it_r in
+    (**) elim_reverse_inv_vp1 p rs r_f r_r;
+    (**) mlistN_entry_null_iff p r_f;
+    let r_f' = listN_next p r_f in
+    (p.cell r_f).write_next r_r;
+    write it_f r_f';
+    write it_r r_f;
+    (**) intro_mlistN_cons p r_f r_r;
+    (**) intro_reverse_inv p trg it_f it_r (not (is_null r_f')) r_f' r_f;
+    (**) intro_exists (G.hide (not (is_null r_f'))) (reverse_inv p trg it_f it_r)
+
+inline_for_extraction noextract
+let reverse (p : list_param) (r : ref p.r)
+  : Steel (ref p.r)
+          (mlistN p r) (fun rt -> mlistN p rt)
+          (requires fun _ -> True)
+          (ensures fun h0 rt h1 -> sel_listN p rt h1 == L.rev (sel_listN p r h0))
+  =
+    (**) let l0 : G.erased (mlistN_sel_t p r) = gget (mlistN p r) in
+    (**) let trg = G.hide (L.rev l0) in
+    let it_f = malloc #(ref p.r) r    in
+    let it_r = malloc #(ref p.r) null in
+    (**) intro_mlistN_nil p null;
+    (**) intro_reverse_inv p trg it_f it_r (not (is_null r)) r null;
+    (**) intro_exists (G.hide (not (is_null r))) (reverse_inv p trg it_f it_r);
+    Loops.while_loop (reverse_inv p trg it_f it_r)
+                     (reverse_loop_cond p trg it_f it_r)
+                     (reverse_loop_body p trg it_f it_r);
+    (**) let rs = elim_reverse_inv p trg it_f it_r false in
+    let r_r = read it_r in
+    (**) elim_reverse_inv_vp1 p rs null r_r;
+    (**) elim_mlistN_nil p null;
+    free it_f;
+    free it_r;
+    r_r
+
+(* ------------------------------------------------- *)
+
+#push-options "--__no_positivity"
+noeq
+type cell = {
+  next: ref cell;
+  data_x: U32.t;
+  data_y: bool
+}
+#pop-options
+
+inline_for_extraction noextract
+let p : list_param =
+  list_param_of_vptr cell (U32.t & bool)
+    ({get = (fun c -> c.next); set = (fun c x -> {c with next = x})})
+    (fun c   -> (c.data_x, c.data_y))
+
+let rec p_length (r : ref cell)
+  : Steel  U32.t
+          (mlistN p r) (fun _ -> mlistN p r)
+          (requires fun h0        -> L.length (sel_listN p r h0) <= FStar.UInt.max_int U32.n)
+          (ensures  fun h0 len h1 -> frame_equalities (mlistN p r) h0 h1 /\
+                                  U32.v len = L.length (sel_listN p r h0))
+  = length_body p p_length r
+
+noextract
+let p_reverse (r : ref cell)
+  : Steel (ref cell)
+          (mlistN p r) (fun rt -> mlistN p rt)
+          (requires fun _ -> True)
+          (ensures fun h0 rt h1 -> sel_listN p rt h1 == L.rev (sel_listN p r h0))
+  = reverse p r
